\documentclass[12pt,fleqn]{exam}
\usepackage{amsmath}
\setlength{\mathindent}{0pt}
\usepackage{amssymb}


\title{ML Assignment 1}
\author{Shubham Sanghavi}
\date{\today}


\begin{document}

   \begin{flushleft}
      \textit{CS 6375 Spring 2020}\\
      \Large\textbf{Problem Set 1}\\
   \end{flushleft}

\begin{flushleft}
Netid: SAS19003\\
Name: Shubham Sanghavi\\
Email: shubham.sanghavi@utdallas.edu\\
\end{flushleft}


\section*{Warm-Up : Subgradients and More}
\begin{enumerate}
    \item Recall that a function $f: \mathbb{R}^n \rightarrow \mathbb{R}$ is convex for all $x,y \in \mathbb{R}^n$ and $\lambda \in [0,1], if \\ \lambda f(x)+ (1-\lambda)f(y) \geq f(\lambda x + (1-\lambda)y)$. Using this definition, show that
    \begin{enumerate}
    \item $f(x) = w f_1(x)$ is a convex function for $ x \in \mathbb{R}^n$ whenever $f_1: \mathbb{R}^n \rightarrow \mathbb{R}$ is a convex function and $ w \geq 0$\\ \\
    \textbf{Ans:}
    {\setlength{\abovedisplayskip}{0pt}
    \begin{flalign*}
        &\lambda f(x)+ (1-\lambda)f(y)\\
        =\quad &\lambda w f_1(x) + ( 1 - \lambda)w f_1(y) 
        \ \ \ \ [ \ \because f(x) = w f_1(x) \ ]\\
        =\quad &w (\lambda f_1(x)+ (1-\lambda)f_1(y))\\
        \geq \quad &w f_1(\lambda x + (1-\lambda)y)\\
        & \qquad [ \ \because w \geq 0 \qquad \text {and} \\
        & \qquad \ \because f_1 \  \text{is a convex function}\\
        & \qquad \qquad \Longleftrightarrow \lambda f_1(x)+ (1-\lambda)f_1(y) \geq f_1(\lambda x + (1-\lambda)y) \ ]\\
        = \quad & f( \lambda x + ( 1 - \lambda) y )\\
        \therefore \quad & \lambda f(x)+ (1-\lambda)f(y) \geq f(\lambda x + (1-\lambda)y\\
        \therefore \quad & f \ \text{is a convex function}
    \end{flalign*}}
    \item $f(x) = f_1(x) + f_2(x) $ is a convex function for $ x \in \mathbb{R}^n$ whenever $f_1: \mathbb{R}^n \rightarrow \mathbb{R}$ and $f_2: \mathbb{R}^n \rightarrow \mathbb{R}$ are convex functions\\ \\
    \textbf{Ans:}
    {\setlength{\abovedisplayskip}{0pt}
    \begin{flalign*}
        &\lambda f(x)+ (1-\lambda)f(y)\\
        = \quad &\lambda (f_1(x) + f_2(x)) + (1-\lambda) (f_1(y) + f_2(y))\\
        = \quad &\lambda f_1(x) + (1-\lambda) f_1(y) + \lambda f_2(x) +  (1-\lambda) f_2(y)\\
        \geq \quad & f_1(\lambda x + ( 1 - \lambda) y) + f_2( \lambda x + ( 1 - \lambda) y)\\
        & \qquad [ \ \because f_1 \ \text{and} \ f_2 \ \text{are convex functions} \ ]\\
        = \quad & f( \lambda x + ( 1 - \lambda) y )\\
        \therefore \quad & \lambda f(x)+ (1-\lambda)f(y) \geq f(\lambda x + (1-\lambda)y\\
        \therefore \quad & f \ \text{is a convex function}
    \end{flalign*}}
    \item $f(x) = max\{f_1(x),f_2(x)\} $ is a convex function for $ x \in \mathbb{R}^n$ whenever $f_1: \mathbb{R}^n \rightarrow \mathbb{R}$ and $f_2: \mathbb{R}^n \rightarrow \mathbb{R}$ are convex functions\\ \\
    \textbf{Ans:}
    {\setlength{\abovedisplayskip}{0pt}
    \begin{flalign*}
        &\lambda f(x)+ (1-\lambda)f(y)\\
        = \quad & \lambda \  max\{f_1(x),f_2(x)\} + ( 1 - \lambda) \  max\{f_1(y),f_2(y)\}\\
        \geq \quad & \lambda f_1(x) + ( 1 - \lambda) f_1(y) \qquad \qquad \text {and} \qquad \qquad \geq  \quad \lambda f_2(x) + ( 1 - \lambda) f_2(y)\\
        & \qquad [ \ \because \ max\{f_1(x),f_2(x)\} \geq f_1(x) \ ] \qquad  \qquad  \qquad [\ \because \ max\{f_1(x),f_2(x)\} \geq f_2(x) \ ]\\
        \geq \quad & f_1(\lambda x + (1-\lambda) y) \qquad \qquad \qquad \text{and} \qquad \qquad \geq \quad  f_2(\lambda x + (1-\lambda) y) \\
        & \qquad [ \ \because \ f_1 \text{ is a convex function} \ ] \qquad  \qquad \qquad \qquad [\ \because \ f_2 \text{ is a convex function} \ ]\\
        \Leftrightarrow \quad &  \lambda f(x)+ (1-\lambda)f(y) \geq max\{f_1(\lambda x + (1-\lambda) y),f_2(\lambda x + (1-\lambda) y)\}\\
        \Leftrightarrow \quad &  \lambda f(x)+ (1-\lambda)f(y) \geq f(\lambda x + (1-\lambda) y)\\
        \therefore \quad & f \ \text{is a convex function}
    \end{flalign*}}

    \end{enumerate}

    
\end{enumerate}

\end{document}